Access.v
@@ -1,0 +1,126 @@
+From Elo Require Import Array.
+From Elo Require Import Core0.
+
+Inductive access (m : mem) : tm -> addr -> Prop :=
+  | access_mem : forall ad ad',
+    access m (getTM m ad') ad ->
+    access m (TM_Loc ad') ad
+
+  | access_loc : forall ad,
+    access m (TM_Loc ad) ad
+
+  | access_new : forall t ad,
+    access m t ad ->
+    access m (TM_New t) ad
+
+  | access_load : forall t ad,
+    access m t ad ->
+    access m (TM_Load t) ad
+
+  | access_asg1 : forall l r ad,
+    access m l ad ->
+    access m (TM_Asg l r) ad
+
+  | access_asg2 : forall l r ad,
+    access m r ad ->
+    access m (TM_Asg l r) ad
+
+  | access_seq1 : forall t1 t2 ad,
+    access m t1 ad ->
+    access m (TM_Seq t1 t2) ad
+
+  | access_seq2 : forall t1 t2 ad,
+    access m t2 ad ->
+    access m (TM_Seq t1 t2) ad
+  .
+
+(* strong access_mem *)
+Theorem access_get_trans : forall m t ad ad',
+  access m t ad' ->
+  access m (getTM m ad') ad ->
+  access m t ad.
+Proof.
+  intros * Hacc ?. induction Hacc; eauto using access.
+Qed.
+
+Ltac inversion_access :=
+  match goal with
+    | [ H : access _ TM_Nil _ |- _ ] => inversion H; clear H
+    | [ H : access _ (TM_Num _) _ |- _ ] => inversion H; clear H
+    | [ H : access _ (TM_New _) _ |- _ ] => inversion H; subst; clear H
+    | [ H : access _ (TM_Load _) _ |- _ ] => inversion H; subst; clear H
+    | [ H : access _ (TM_Asg _ _) _ |- _ ] => inversion H; subst; clear H
+    | [ H : access _ (TM_Seq _ _) _ |- _ ] => inversion H; subst; clear H
+  end.
+
+Lemma inversion_not_access_new : forall m t ad,
+  ~ access m (TM_New t) ad ->
+  ~ access m t ad.
+Proof.
+  intros * ? F. inversion F; subst; eauto using access.
+Qed.
+
+Lemma inversion_not_access_load : forall m t ad,
+  ~ access m (TM_Load t) ad ->
+  ~ access m t ad.
+Proof.
+  intros * ? F. inversion F; subst; eauto using access.
+Qed.
+
+Lemma inversion_not_access_asg : forall m l r ad,
+  ~ access m (TM_Asg l r) ad ->
+  ~ access m l ad /\ ~ access m r ad.
+Proof.
+  intros * ?. split; intros F; inversion F; subst; eauto using access.
+Qed.
+
+Lemma inversion_not_access_seq : forall m t1 t2 ad,
+  ~ access m (TM_Seq t1 t2) ad ->
+  ~ access m t1 ad /\ ~ access m t2 ad.
+Proof.
+  intros * ?. split; intros F; inversion F; subst; eauto using access.
+Qed.
+
+Ltac inversion_not_access :=
+  match goal with
+    | [ H : ~ access _ (TM_New _) _ |- _ ] =>
+        eapply inversion_not_access_new in H; clear H
+    | [ H : ~ access _ (TM_Load _) _ |- _ ] =>
+        eapply inversion_not_access_load in H; clear H
+    | [ H : ~ access _ (TM_Asg _ _) _ |- _ ] =>
+        eapply inversion_not_access_asg in H; clear H
+    | [ H : ~ access _ (TM_Seq _ _) _ |- _ ] =>
+        eapply inversion_not_access_seq in H; clear H
+  end.
+
+Lemma access_load_not : forall m t ad,
+  ~ access m t ad ->
+  ~ access m (TM_Load t) ad.
+Proof.
+  intros * ? ?. inversion_access. eauto.
+Qed.
+
+Lemma access_asg_not : forall m l r ad,
+  ~ access m l ad /\ ~ access m r ad ->
+  ~ access m (TM_Asg l r) ad.
+Proof.
+  intros * [? ?] ?. inversion_access; eauto.
+Qed.
+
+Lemma access_seq_not : forall m t1 t2 ad,
+  ~ access m t1 ad /\ ~ access m t2 ad ->
+  ~ access m (TM_Seq t1 t2) ad.
+Proof.
+  intros * [? ?] ?. inversion_access; eauto.
+Qed.
+
+
+(*
+Ltac destruct_access_H H :=
+  idtac H;
+  match type of H with
+    | access _ TM_Nil _ => inversion H
+    | access _ (TM_Num _) _ => inversion H
+    | access _ (TM_New _) _ => eapply new_access in H
+  end.
+*)
