Compat.v
@@ -1,0 +1,82 @@
+From Coq Require Import Arith.Arith.
+
+From Elo Require Import Array.
+From Elo Require Import Core0.
+From Elo Require Import Access.
+
+Definition compat m m' t := forall ad,
+  access m t ad ->
+  getTM m ad = getTM m' ad.
+
+Lemma compat_symmetry : forall m m' t, 
+  compat m m' t ->
+  compat m' m t. 
+Proof.
+  intros * Hcompat ad Hacc. unfold compat in *.
+  induction Hacc; eauto using access;
+  try solve [symmetry; eauto using access].
+  eapply IHHacc. intros ? ?.
+  eapply Hcompat. eapply access_mem.
+  rewrite (Hcompat _ (access_loc _ _)).
+  trivial.
+Qed.
+
+Local Lemma compat_access : forall m m' t ad,
+  compat m m' t ->
+  access m t ad ->
+  access m' t ad.
+Proof.
+  intros * Hcompat Hacc. unfold compat in *.
+  induction Hacc; eauto using access.
+  eapply access_mem.
+  rewrite <- (Hcompat _ (access_loc _ _)).
+  eapply IHHacc. intros ? ?.
+  eapply Hcompat. eauto using access.
+Qed.
+
+Lemma compat_access_symmetry : forall m m' t ad,
+  compat m m' t ->
+  access m t ad <-> access m' t ad.
+Proof.
+  intros * ?. split; eauto using compat_access, compat_symmetry.
+Qed.
+
+Lemma compat_set : forall m m' t ad v,
+  compat m m' t ->
+  ~ access m t ad ->
+  compat m (set m' ad v) t.
+Proof.
+  intros * Hcompat Hnacc ad Hacc. unfold compat in *.
+  induction Hacc. 
+  - eapply IHHacc; eauto using access.
+  - match goal with H : ~ access _ _ ?ad' |- _ => 
+      destruct (Nat.eq_dec ad ad'); subst
+    end.
+    + exfalso. eauto using access.
+    + rewrite (get_set_neq TM_Nil); eauto using access.
+  - eauto using access, inversion_not_access_new.
+  - eauto using access, inversion_not_access_load.
+  - eapply inversion_not_access_asg in Hnacc as [? ?]. eauto using access.
+  - eapply inversion_not_access_asg in Hnacc as [? ?]. eauto using access.
+  - eapply inversion_not_access_seq in Hnacc as [? ?]. eauto using access.
+  - eapply inversion_not_access_seq in Hnacc as [? ?]. eauto using access.
+Qed.
+
+Lemma
+  access m t ad ->
+  ~ access m t ad' ->
+  access (set m ad' v) t ad.
+Usar o de cima.
+  
+
+Def NonInterf m ths := forall tid1 tid2 ad,
+  access m (get tid1) ad ->
+  access m (get tid2) ad ->
+  tid1 = tid2.
+
+
+Lemma  noninterf_preservation
+  has_type t // sí
+  noninter t
+  t --> t'
+  noninter t'
