Makefile
@@ -6,7 +6,7 @@ main:
 	$(COQC) Array.v
 	$(COQC) Map.v
 	$(COQC) Core0.v
-	$(COQC) Safety.v
+	$(COQC) Access.v
 
 clean:
 	rm -f *.vo *.vok *.vos *.glob
